src/FcEtt/toplevel.v
@@ -26,7 +26,7 @@ Qed.
 (* ------------------------------------------ *)
 
 (* Tactics for working with 'binds' assumptions in the context. *)
-Ltac binds_case IHst :=
+Ltac binds_case :=
   intros;
   match goal with
   | [ H : binds ?F ?s nil |- _ ] => inversion H
@@ -35,26 +35,18 @@ Ltac binds_case IHst :=
       match goal with [ H3 : (_,_) = (_,_) |- _ ] => inversion H3;
       subst; try split; eauto end
     | (* bound elsewhere *)
-      eapply IHst; eauto]
+      eauto]
   end.
 
 Lemma toplevel_closed : forall F a A, binds F (Ax a A) toplevel -> Typing nil a A.
 Proof.
   have st: Sig toplevel by apply Sig_toplevel.
   induction st.
-  all: binds_case IHst.
-Qed.
-
-
-Lemma toplevel_to_const : forall T A, binds T (Cs A) toplevel -> Typing nil A a_Star.
-Proof.
-  have st: Sig toplevel by apply Sig_toplevel.
-  induction st.
-  all: binds_case IHst.
+  all: binds_case.
 Qed.
 
 (*
-Lemma toplevel_to_datacon : forall K A T, binds K (Dc A T) toplevel -> Typing nil A a_Star /\ exists B, DataTy A B /\ Path T B.
+Lemma toplevel_to_const : forall T A, binds T (Cs A) toplevel -> Typing nil A a_Star.
 Proof.
   have st: Sig toplevel by apply Sig_toplevel.
   induction st.
@@ -62,34 +54,48 @@ Proof.
 Qed.
 *)
 
+Lemma toplevel_to_const :
+  forall K A a, binds K (Cs A a) toplevel ->
+           Typing nil A a_Star /\ exists B, DataTy A B /\ Constr B.
+Proof.
+  have st: Sig toplevel by apply Sig_toplevel.
+  induction st.
+  all: binds_case.
+Qed.
+
+
 
 Lemma an_toplevel_closed : forall F a A, binds F (Ax a A) an_toplevel ->
                                     AnnTyping nil a A.
 Proof.
   have st: AnnSig an_toplevel by apply AnnSig_an_toplevel.
   induction st.
-  all: binds_case IHst.
+  all: binds_case.
 Qed.
 
-Lemma an_toplevel_to_const : forall T A, binds T (Cs A) an_toplevel -> AnnTyping nil A a_Star.
+(*
+Lemma an_toplevel_to_const : forall T A, binds T (Cs A) an_toplevel ->
+                                    AnnTyping nil A a_Star.
 Proof.
   have st: AnnSig an_toplevel by apply AnnSig_an_toplevel.
   induction st.
-  all: binds_case IHst.
+  all: binds_case.
 Qed.
-
-
+*)
+(*
 Lemma binds_to_type : forall T A, binds T (Cs A) an_toplevel -> DataTy A a_Star.
 Proof.
   have st: AnnSig an_toplevel by apply AnnSig_an_toplevel.
   induction st.
-  all: binds_case IHst.
+  all: binds_case.
 Qed.
+*)
 
-
-Lemma an_toplevel_to_datacon : forall K A T, binds K (Dc A T) an_toplevel -> AnnTyping nil A a_Star /\ exists B, DataTy A B /\ Path T B.
+Lemma an_toplevel_to_const :
+  forall K A a, binds K (Cs A a) an_toplevel ->
+           AnnTyping nil A a_Star /\ exists B, DataTy A B /\ Constr B.
 Proof.
   have st: AnnSig an_toplevel by apply AnnSig_an_toplevel.
   induction st.
-  all: binds_case IHst.
+  all: binds_case.
 Qed.
